ulib/FStar.Class.Embeddable.fsti
@@ -10,6 +10,6 @@ class embeddable (a:Type) = {
 instance val embeddable_string : embeddable string
 instance val embeddable_bool   : embeddable bool
 instance val embeddable_int    : embeddable int
+instance val embeddable_bv_t (n:nat) : embeddable (FStar.BV.bv_t n)
 
 instance val embeddable_list (a:Type) (ea : embeddable a) : embeddable (list a)
-instance val embeddable_bv (n:nat) : embeddable (FStar.BV.bv_t n)
